Refactoring and renamings in Spec.Blake2s to be consistant with implementation

specs/Spec.Blake2s.fst
@@ -23,7 +23,7 @@ type counter = uint64
 type last_block_flag = bool
 
 noeq type state = {
-  h: hash_state;
+  s: hash_state;
   t: intseq U32 2;
   f: intseq U32 2;
   buf: intseq U8 size_block;
@@ -76,143 +76,143 @@ let const_sigma:lseq (n:size_t{size_v n < 16}) 160 =
 
 
 (* Functions *)
-let g1 (v: working_vector) (a:idx) (b:idx) (r:rotval U32) : Tot working_vector =
-  v.[a] <- (v.[a] ^. v.[b]) >>>. r
+let g1 (wv: working_vector) (a:idx) (b:idx) (r:rotval U32) : Tot working_vector =
+  wv.[a] <- (wv.[a] ^. wv.[b]) >>>. r
 
-let g2 (v:working_vector) (a:idx) (b:idx) (x:uint32) : Tot working_vector =
-  v.[a] <- (v.[a] +. v.[b] +. x)
+let g2 (wv:working_vector) (a:idx) (b:idx) (x:uint32) : Tot working_vector =
+  wv.[a] <- (wv.[a] +. wv.[b] +. x)
 
 
 val blake2_mixing : working_vector -> idx -> idx -> idx -> idx -> uint32 -> uint32 -> Tot working_vector
-let blake2_mixing v a b c d x y =
-  let v = g2 v a b x in
-  let v = g1 v d a r1 in
-  let v = g2 v c d (u32 0) in
-  let v = g1 v b c r2 in
-  let v = g2 v a b y in
-  let v = g1 v d a r3 in
-  let v = g2 v c d (u32 0) in
-  let v = g1 v b c r4 in
-  v
+let blake2_mixing wv a b c d x y =
+  let wv = g2 wv a b x in
+  let wv = g1 wv d a r1 in
+  let wv = g2 wv c d (u32 0) in
+  let wv = g1 wv b c r2 in
+  let wv = g2 wv a b y in
+  let wv = g1 wv d a r3 in
+  let wv = g2 wv c d (u32 0) in
+  let wv = g1 wv b c r4 in
+  wv
 
 
 val blake2_round1 : working_vector -> message_block -> size_nat -> Tot working_vector
-let blake2_round1 v m i =
+let blake2_round1 wv m i =
   let s = sub const_sigma ((i % 10) * 16) 16 in
-  let v = blake2_mixing v 0 4  8 12 (m.[size_v s.[ 0]]) (m.[size_v s.[ 1]]) in
-  let v = blake2_mixing v 1 5  9 13 (m.[size_v s.[ 2]]) (m.[size_v s.[ 3]]) in
-  let v = blake2_mixing v 2 6 10 14 (m.[size_v s.[ 4]]) (m.[size_v s.[ 5]]) in
-  let v = blake2_mixing v 3 7 11 15 (m.[size_v s.[ 6]]) (m.[size_v s.[ 7]]) in
-  v
+  let wv = blake2_mixing wv 0 4  8 12 (m.[size_v s.[ 0]]) (m.[size_v s.[ 1]]) in
+  let wv = blake2_mixing wv 1 5  9 13 (m.[size_v s.[ 2]]) (m.[size_v s.[ 3]]) in
+  let wv = blake2_mixing wv 2 6 10 14 (m.[size_v s.[ 4]]) (m.[size_v s.[ 5]]) in
+  let wv = blake2_mixing wv 3 7 11 15 (m.[size_v s.[ 6]]) (m.[size_v s.[ 7]]) in
+  wv
 
 
 val blake2_round2 : working_vector -> message_block -> size_nat -> Tot working_vector
-let blake2_round2 v m i =
+let blake2_round2 wv m i =
   let s = sub const_sigma ((i % 10) * 16) 16 in
-  let v = blake2_mixing v 0 5 10 15 (m.[size_v s.[ 8]]) (m.[size_v s.[ 9]]) in
-  let v = blake2_mixing v 1 6 11 12 (m.[size_v s.[10]]) (m.[size_v s.[11]]) in
-  let v = blake2_mixing v 2 7  8 13 (m.[size_v s.[12]]) (m.[size_v s.[13]]) in
-  let v = blake2_mixing v 3 4  9 14 (m.[size_v s.[14]]) (m.[size_v s.[15]]) in
-  v
+  let wv = blake2_mixing wv 0 5 10 15 (m.[size_v s.[ 8]]) (m.[size_v s.[ 9]]) in
+  let wv = blake2_mixing wv 1 6 11 12 (m.[size_v s.[10]]) (m.[size_v s.[11]]) in
+  let wv = blake2_mixing wv 2 7  8 13 (m.[size_v s.[12]]) (m.[size_v s.[13]]) in
+  let wv = blake2_mixing wv 3 4  9 14 (m.[size_v s.[14]]) (m.[size_v s.[15]]) in
+  wv
 
 
 val blake2_round : message_block -> size_nat -> working_vector -> Tot working_vector
-let blake2_round m i v =
-  let v = blake2_round1 v m i in
-  let v = blake2_round2 v m i in
-  v
+let blake2_round m i wv =
+  let wv = blake2_round1 wv m i in
+  let wv = blake2_round2 wv m i in
+  wv
 
 
 val blake2_compress1 : working_vector -> hash_state -> message_block -> uint64 -> last_block_flag -> Tot working_vector
-let blake2_compress1 v h m offset flag =
-  let v = update_sub v 0 8 h in
-  let v = update_sub v 8 8 const_iv in
+let blake2_compress1 wv s m offset flag =
+  let wv = update_sub wv 0 8 s in
+  let wv = update_sub wv 8 8 const_iv in
   let low_offset = to_u32 #U64 offset in
   let high_offset = to_u32 #U64 (offset >>. u32 32) in
-  let v_12 = v.[12] ^. low_offset in
-  let v_13 = v.[13] ^. high_offset in
-  let v_14 = v.[14] ^. (u32 0xFFFFFFFF) in
-  let v = v.[12] <- v_12 in
-  let v = v.[13] <- v_13 in
-  let v = if flag then v.[14] <- v_14 else v in
-  v
+  let wv_12 = wv.[12] ^. low_offset in
+  let wv_13 = wv.[13] ^. high_offset in
+  let wv_14 = wv.[14] ^. (u32 0xFFFFFFFF) in
+  let wv = wv.[12] <- wv_12 in
+  let wv = wv.[13] <- wv_13 in
+  let wv = if flag then wv.[14] <- wv_14 else wv in
+  wv
 
 
 val blake2_compress2: working_vector -> message_block -> Tot working_vector
-let blake2_compress2 v m = repeati rounds_in_f (blake2_round m) v
+let blake2_compress2 wv m = repeati rounds_in_f (blake2_round m) wv
 
 
 val blake2_compress3_inner: working_vector -> i:size_nat{i < 8} -> hash_state -> Tot hash_state
-let blake2_compress3_inner v i h =
+let blake2_compress3_inner wv i s =
   let i_plus_8 = i + 8 in
-  let hi_xor_wvi = logxor #U32 h.[i] v.[i] in
-  let hi = logxor #U32 hi_xor_wvi v.[i_plus_8] in
-  h.[i] <- hi
+  let si_xor_wvi = logxor #U32 s.[i] wv.[i] in
+  let si = logxor #U32 si_xor_wvi wv.[i_plus_8] in
+  s.[i] <- si
 
 
 val blake2_compress3: working_vector -> hash_state -> Tot hash_state
-let blake2_compress3 v h = repeati 8 (blake2_compress3_inner v) h
+let blake2_compress3 wv s = repeati 8 (blake2_compress3_inner wv) s
 
 
 val blake2_compress : hash_state -> message_block -> uint64 -> last_block_flag -> Tot hash_state
-let blake2_compress h m offset flag =
-  let v = create 16 (u32 0) in
-  let v = blake2_compress1 v h m offset flag in
-  let v = blake2_compress2 v m in
-  let h = blake2_compress3 v h in
-  h
+let blake2_compress s m offset flag =
+  let wv = create 16 (u32 0) in
+  let wv = blake2_compress1 wv s m offset flag in
+  let wv = blake2_compress2 wv m in
+  let s = blake2_compress3 wv s in
+  s
 
 
 // Init
-val blake2s_internal1 : h:intseq U32 8 -> kk:size_nat{kk<=32} -> nn:size_nat{1 <= nn /\ nn <= 32} -> Tot (intseq U32 8)
-let blake2s_internal1 h kk nn =
-  let h0 = h.[0] in
-  let h0' = h0 ^. (u32 0x01010000) ^. ((u32 kk) <<. (u32 8)) ^. (u32 nn) in
-  h.[0] <- h0'
+val blake2s_internal1: hash_state -> kk:size_nat{kk<=32} -> nn:size_nat{1 <= nn /\ nn <= 32} -> Tot hash_state
+let blake2s_internal1 s kk nn =
+  let s0 = s.[0] in
+  let s0' = s0 ^. (u32 0x01010000) ^. ((u32 kk) <<. (u32 8)) ^. (u32 nn) in
+  s.[0] <- s0'
 
 
 // Update 1
-val blake2s_internal2_inner: dd:size_nat{0 < dd /\ dd * size_block <= max_size_t} -> d:lbytes (dd * size_block) -> i:size_nat{i < dd - 1} -> h:intseq U32 8 -> Tot (h:intseq U32 8)
-let blake2s_internal2_inner dd d i h =
+val blake2s_internal2_inner: dd:size_nat{0 < dd /\ dd * size_block <= max_size_t} -> d:lbytes (dd * size_block) -> i:size_nat{i < dd - 1} -> hash_state -> Tot hash_state
+let blake2s_internal2_inner dd d i s =
   let sub_d = (sub d (i * size_block) size_block) in
   let to_compress : intseq U32 16 = uints_from_bytes_le sub_d in
   let offset = u64 ((i + 1) * size_block) in
-  blake2_compress h to_compress offset false
+  blake2_compress s to_compress offset false
 
 
 // Update_blocks // Update_multi
-val blake2s_internal2_loop : dd:size_nat{0 < dd /\ dd * size_block <= max_size_t} -> d:lbytes (dd * size_block) -> h:intseq U32 8 -> Tot (h:intseq U32 8)
-let blake2s_internal2_loop dd d h = repeati (dd - 1) (blake2s_internal2_inner dd d) h
+val blake2s_internal2_loop : dd:size_nat{0 < dd /\ dd * size_block <= max_size_t} -> d:lbytes (dd * size_block) -> hash_state -> Tot hash_state
+let blake2s_internal2_loop dd d s = repeati (dd - 1) (blake2s_internal2_inner dd d) s
 
 
 // BB. This seems odd as blake2 internal should be called when dd = 1 !!
-val blake2s_internal2 : dd:size_nat{0 < dd /\ dd * size_block <= max_size_t} -> d:lbytes (dd * size_block) -> h:intseq U32 8 -> Tot (h:intseq U32 8)
-let blake2s_internal2 dd d h =
+val blake2s_internal2 : dd:size_nat{0 < dd /\ dd * size_block <= max_size_t} -> d:lbytes (dd * size_block) -> hash_state -> Tot hash_state
+let blake2s_internal2 dd d s =
   if dd > 1 then
-    blake2s_internal2_loop dd d h
-  else h
+    blake2s_internal2_loop dd d s
+  else s
 
 
 // Update last
 // We should insert the key in update1 instead ?
-val blake2s_internal3 : h:intseq U32 8 -> dd:size_nat{0 < dd /\ dd * size_block <= max_size_t} -> d:lbytes (dd * size_block) -> ll:size_nat -> kk:size_nat{kk<=32} -> nn:size_nat{1 <= nn /\ nn <= 32} -> Tot hash_state
+val blake2s_internal3 : hash_state -> dd:size_nat{0 < dd /\ dd * size_block <= max_size_t} -> d:lbytes (dd * size_block) -> ll:size_nat -> kk:size_nat{kk<=32} -> nn:size_nat{1 <= nn /\ nn <= 32} -> Tot hash_state
 
-let blake2s_internal3 h dd d ll kk nn =
+let blake2s_internal3 s dd d ll kk nn =
   let offset : size_nat = (dd - 1) * 16 * 4 in
   let last_block : intseq U32 16 = uints_from_bytes_le (sub d offset size_block) in
   if kk = 0 then
-    blake2_compress h last_block (u64 ll) true
+    blake2_compress s last_block (u64 ll) true
   else
-    blake2_compress h last_block (u64 (ll + size_block)) true
+    blake2_compress s last_block (u64 (ll + size_block)) true
 
 
 val blake2s_internal_core : dd:size_nat{0 < dd /\ dd * size_block <= max_size_t} -> d:lbytes (dd * size_block) -> ll:size_nat -> kk:size_nat{kk<=32} -> nn:size_nat{1 <= nn /\ nn <= 32} -> Tot (lseq uint8 32)
 let blake2s_internal_core dd d ll kk nn =
-  let h = const_iv in
-  let h = blake2s_internal1 h kk nn in
-  let h = blake2s_internal2 dd d h in
-  let h = blake2s_internal3 h dd d ll kk nn in
-  uints_to_bytes_le h
+  let s = const_iv in
+  let s = blake2s_internal1 s kk nn in
+  let s = blake2s_internal2 dd d s in
+  let s = blake2s_internal3 s dd d ll kk nn in
+  uints_to_bytes_le s
 
 
 val blake2s_internal : dd:size_nat{0 < dd /\ dd * size_block <= max_size_t} -> d:lbytes (dd * size_block) -> ll:size_nat -> kk:size_nat{kk<=32} -> nn:size_nat{1 <= nn /\ nn <= 32} -> Tot (lbytes nn)
